cclc

coq/cclc/cclc_eval.v
@@ -1,6 +1,9 @@
 From mathcomp Require Import ssreflect ssrbool eqtype ssrnat seq.
-From Coq Require Import ssrfun Classical Utf8.
-Require Import AutosubstSsr ARS clc_context clc_ast.
+From Coq Require Import ssrfun Utf8 Classical.
+Require Import AutosubstSsr ARS 
+  clc_context clc_ast clc_confluence clc_subtype clc_typing
+  clc_weakening clc_substitution clc_inversion clc_validity
+  clc_soundness clc_eval clc_linearity.
 
 Set Implicit Arguments.
 Unset Strict Implicit.
@@ -20,7 +23,6 @@ Inductive value : term -> Prop :=
 
 Inductive eval_context :=
 | EHole : eval_context
-| EVar : var -> eval_context
 | EAppL : eval_context -> term -> eval_context
 | EAppR m : value m -> eval_context -> eval_context
 | EPairL : eval_context -> term -> sort -> eval_context
@@ -40,7 +42,6 @@ Local Open Scope eval_scope.
 Fixpoint plug (e : eval_context) (t : term) : term :=
   match e with
   | EHole => t
-  | EVar x => Var x
   | EAppL e m => App (plug e t) m
   | EAppR m _ e => App m (plug e t)
   | EPairL e m s => Pair (plug e t) m s
@@ -56,3 +57,259 @@ Fixpoint plug (e : eval_context) (t : term) : term :=
 Notation "c .[ m ] " := (plug c m)
   (at level 2, m at level 200, left associativity,
     format "c .[ m ]") : eval_scope.
+
+Lemma plug_inv Γ c m A s : 
+  ok Γ -> Γ ⊢ c.[m] : A : s -> 
+  exists Γ1 Γ2 B t,
+    Γ1 ∘ Γ2 => Γ /\
+    Γ1 ⊢ m : B : t /\
+    (~Γ1 |> U ->
+    forall Γ3 Γ' n,
+      Γ3 ∘ Γ2 => Γ' ->
+      Γ3 ⊢ n : B : t ->
+      Γ' ⊢ c.[n] : A : s).
+Proof with eauto using clc_type, merge_reR, merge_pure.
+  move e:(c.[m])=>n wf ty. 
+  elim: ty wf c m e=>{Γ n A s}.
+  move=>Γ s l k wf c m e.
+  { destruct c; simpl in e; inv e.
+    exists Γ. exists Γ.  exists (U @ l.+1). exists U.
+    repeat split...
+    move=>//. }
+  move=>Γ A B s r t i k tyA _ tyB _ wf c m e.
+  { destruct c; simpl in e; inv e.
+    exists Γ. exists Γ. exists (t @ i). exists U.
+    repeat split...
+    move=>//. }
+  move=>Γ x A s hs wf c m e.
+  { destruct c; simpl in e; inv e.
+    exists Γ. exists [Γ]. exists A. exists s.
+    repeat split...
+    move=>k Γ3 Γ' n mrg tyn//=.
+    have->//:=merge_pureR mrg (re_pure _). }
+  move=>Γ A B m s r t i k tyP _ tym _ wf c m0 e.
+  { destruct c; simpl in e; inv e.
+    exists Γ. exists [Γ]. exists (Pi A B s r t). exists t.
+    repeat split...
+    move=>k' Γ3 Γ' n mrg tyn//=.
+    have->//:=merge_pureR mrg (re_pure _). }
+  move=>Γ1 Γ2 Γ A B m n s r t k mrg tym ihm tyn ihn wf c m0 e.
+  { destruct c; simpl in e; inv e.
+    { exists Γ. exists [Γ]. exists B.[n/]. exists r.
+      repeat split...
+      move=>k' Γ3 Γ' n0 mrg' tyn0//=.
+      have->//:=merge_pureR mrg' (re_pure _). }
+    { have[wf1 wf2]:=merge_context_ok_inv mrg wf.
+      have{ihm ihn}[G1[G2[B0[t0[mrg0[tym0 ih]]]]]]:=ihm wf1 _ _ erefl.
+      have[G3[mrg1 mrg2]]:=merge_splitL mrg (merge_sym mrg0).
+      exists G1. exists G3. exists B0. exists t0.
+      repeat split...
+      apply: merge_sym...
+      move=>k' Γ3 Γ' n0 mrg3 tyn0//=.
+      have[G4[mrg4 mrg5]]:=merge_splitL (merge_sym mrg3) mrg1.
+      have{}ih:=ih k' _ _ _ (merge_sym mrg4) tyn0.
+      econstructor... }
+    { have[wf1 wf2]:=merge_context_ok_inv mrg wf.
+      have{ihm ihn}[G1[G2[B0[t0[mrg0[tym0 ih]]]]]]:=ihn wf2 _ _ erefl.
+      have[G3[mrg1 mrg2]]:=merge_splitL (merge_sym mrg) (merge_sym mrg0).
+      exists G1. exists G3. exists B0. exists t0.
+      repeat split...
+      apply: merge_sym...
+      move=>k' Γ3 Γ' n0 mrg3 tyn0//=.
+      have[G4[mrg4 mrg5]]:=merge_splitL (merge_sym mrg3) mrg1.
+      have{}ih:=ih k' _ _ _ (merge_sym mrg4) tyn0.
+      destruct s.
+      have[]//:=merge_pure_inv mrg0 k.
+      have[lP tyP]:=validity wf1 tym.
+      have[l[tyA[_ tyB]]]:=pi_inv _ _ _ _ _ _ _ _ tyP.
+      have os:of_sort (_: [Γ1]) 0 None by constructor.
+      have oc:=narity tyB os.
+      have->:=nsubst_subst c.[m0] c.[n0] oc.
+      econstructor.
+      apply: (key_impure G4).
+      apply: (merge_sym mrg5).
+      all: eauto. } }
+  move=>Γ k wf c m e.
+  { destruct c; simpl in e; inv e.
+    exists Γ. exists Γ. exists (U @ 0). exists U.
+    repeat split...
+    move=>//. }
+  move=>Γ k wf c m e.
+  { destruct c; simpl in e; inv e.
+    exists Γ. exists Γ. exists Unit. exists U.
+    repeat split...
+    move=>//. }
+  move=>Γ A B s r t i lte k tyA _ tyB _ wf c m e.
+  { destruct c; simpl in e; inv e.
+    exists Γ. exists Γ. exists (t @ i). exists U.
+    repeat split...
+    move=>//. }
+  move=>Γ1 Γ2 Γ A B m n s r t i k1 k2 mrg 
+    tyS ihS tym ihm tyn ihn wf c m0 e.
+  { destruct c; simpl in e; inv e.
+    { exists Γ. exists [Γ]. exists (Sigma A B s r t). exists t.
+      repeat split...
+      move=>k' Γ3 Γ' n0 mrg' tyn0//=.
+      have->//:=merge_pureR mrg' (re_pure _). }
+    { have[wf1 wf2]:=merge_context_ok_inv mrg wf.
+      have{ihm ihn}[G1[G2[B0[t0[mrg0[tym0 ih]]]]]]:=ihm wf1 _ _ erefl.
+      have[G3[mrg1 mrg2]]:=merge_splitL mrg (merge_sym mrg0).
+      exists G1. exists G3. exists B0. exists t0.
+      repeat split...
+      apply: merge_sym...
+      move=>k' Γ3 Γ' n0 mrg3 tyn0//=.
+      have[G4[mrg4 mrg5]]:=merge_splitL (merge_sym mrg3) mrg1.
+      have{}ih:=ih k' _ _ _ (merge_sym mrg4) tyn0.
+      destruct s.
+      have[]//:=merge_pure_inv mrg0 k1.
+      have//=[G5[G6[l[_[mrg6[tyA tyB]]]]]]:=sigma_inv _ _ _ _ _ _ _ tyS.
+      have[_[e1 e2]]:=merge_re_re mrg5.
+      have[_[e3 e4]]:=merge_re_re mrg.
+      econstructor.
+      apply: (key_impure G4).
+      apply: k2.
+      all: eauto.
+      rewrite<-e2. rewrite e4...
+      have os:of_sort (_: [G6]) 0 None by constructor.
+      have oc:=narity tyB os.
+      have->//:=nsubst_subst c.[n0] c.[m0] oc. }
+    { have[wf1 wf2]:=merge_context_ok_inv mrg wf.
+      have{ihm ihn}[G1[G2[B0[t0[mrg0[tym0 ih]]]]]]:=ihn wf2 _ _ erefl.
+      have[G3[mrg1 mrg2]]:=merge_splitL (merge_sym mrg) (merge_sym mrg0).
+      exists G1. exists G3. exists B0. exists t0.
+      repeat split...
+      apply: merge_sym...
+      move=>k' Γ3 Γ' n0 mrg3 tyn0//=.
+      have[G4[mrg4 mrg5]]:=merge_splitL (merge_sym mrg3) mrg1.
+      have{}ih:=ih k' _ _ _ (merge_sym mrg4) tyn0.
+      destruct r.
+      have[]//:=merge_pure_inv mrg0 k2.
+      have[_[e1 e2]]:=merge_re_re mrg5.
+      have[_[e3 e4]]:=merge_re_re mrg.
+      econstructor.
+      apply: k1.
+      apply: (key_impure G4).
+      apply: merge_sym...
+      rewrite<-e2. rewrite e3...
+      all: eauto. } }
+  move=>Γ1 Γ2 Γ m n A s mrg tym ihm tyn _ wf c m0 e.
+  { destruct c; simpl in e; inv e. 
+    { exists Γ. exists [Γ]. exists A. exists s.
+      repeat split...
+      move=>k' Γ3 Γ' m0 mrg0 tym0//=.
+      have->//:=merge_pureR mrg0 (re_pure _). }
+    { have[wf1 wf2]:=merge_context_ok_inv mrg wf.
+      have{ihm}[G1[G2[B0[t0[mrg0[tym0 ih]]]]]]:=ihm wf1 _ _ erefl.
+      have[G3[mrg1 mrg2]]:=merge_splitL mrg (merge_sym mrg0).
+      exists G1. exists G3. exists B0. exists t0.
+      repeat split...
+      apply: merge_sym...
+      move=>k' Γ3 Γ' n0 mrg3 tyn0//=.
+      have[G4[mrg4 mrg5]]:=merge_splitL (merge_sym mrg3) mrg1.
+      have{}ih:=ih k' _ _ _ (merge_sym mrg4) tyn0.
+      econstructor... } }
+  move=>Γ1 Γ2 Γ A B C m n s r t k x i lte key mrg 
+    tym ihm tyC _ tyn _ wf c m0 e.
+  { destruct c; simpl in e; inv e. 
+    { exists Γ. exists [Γ]. exists C.[m/]. exists x.
+      repeat split...
+      move=>k' Γ3 Γ' m0 mrg0 tym0//=.
+      have->//:=merge_pureR mrg0 (re_pure _). }
+    { have[wf1 wf2]:=merge_context_ok_inv mrg wf.
+      have{ihm}[G1[G2[B0[t0[mrg0[tym0 ih]]]]]]:=ihm wf1 _ _ erefl.
+      have[G3[mrg1 mrg2]]:=merge_splitL mrg (merge_sym mrg0).
+      exists G1. exists G3. exists B0. exists t0.
+      repeat split...
+      apply: merge_sym...
+      move=>k' Γ3 Γ' n0 mrg3 tyn0//=.
+      have[G4[mrg4 mrg5]]:=merge_splitL (merge_sym mrg3) mrg1.
+      have{}ih:=ih k' _ _ _ (merge_sym mrg4) tyn0.
+      destruct k.
+      have[]//:=merge_pure_inv mrg0 key.
+      simpl in tyC.
+      have os:of_sort (_: [Γ2]) 0 None by constructor.
+      have oc:=narity tyC os.
+      have->:=nsubst_subst c.[m0] c.[n0] oc.
+      econstructor.
+      exact: lte.
+      apply: (key_impure G4).
+      all: eauto. } }
+  move=>Γ i k wf c m e.
+  { destruct c; simpl in e; inv e.
+    exists Γ. exists Γ. exists (U @ i). exists U.
+    repeat split...
+    move=>//. }
+  move=>Γ i k wf c m e.
+  { destruct c; simpl in e; inv e.
+    exists Γ. exists Γ. exists (Proto 0). exists U.
+    repeat split...
+    move=>//. }
+  move=>Γ i k wf c m e.
+  { destruct c; simpl in e; inv e.
+    exists Γ. exists Γ. exists (Proto 0). exists U.
+    repeat split...
+    move=>//. }
+  move=>Γ A B s i k tyA _ tyB _ wf c m e.
+  { destruct c; simpl in e; inv e.
+    exists Γ. exists Γ. exists (Proto i). exists U.
+    repeat split...
+    move=>//. }
+  move=>Γ A B s i k tyA _ tyB _ wf c m e.
+  { destruct c; simpl in e; inv e.
+    exists Γ. exists Γ. exists (Proto i). exists U.
+    repeat split...
+    move=>//. }
+  move=>Γ A i k tyA ihA wf c m e.
+  { destruct c; simpl in e; inv e.
+    exists Γ. exists Γ. exists (L @ i). exists U.
+    repeat split...
+    move=>//. }
+  move=>Γ A B m s tym ihm wf c m0 e.
+  { destruct c; simpl in e; inv e.
+    { exists Γ. exists [Γ]. exists (Sigma A (Ch B) s L L). exists L.
+      repeat split...
+      move=>k' Γ3 Γ' n mrg tyn//=.
+      have->//:=merge_pureR mrg (re_pure _). }
+    { have{ihm}[G1[G2[B0[t[mrg[tym0 ih]]]]]]:=ihm wf _ _ erefl.
+      exists G1. exists G2. exists B0. exists t.
+      repeat split... } }
+  move=>Γ A B m s tym ihm wf c m0 e.
+  { destruct c; simpl in e; inv e.
+    { exists Γ. exists [Γ]. exists (Pi A (Ch B) s L L). exists L.
+      repeat split...
+      move=>k' Γ3 Γ' n mrg tyn//=.
+      have->//:=merge_pureR mrg (re_pure _). }
+    { have{ihm}[G1[G2[B0[t[mrg[tym0 ih]]]]]]:=ihm wf _ _ erefl.
+      exists G1. exists G2. exists B0. exists t.
+      repeat split... } }
+  move=>Γ m tym ihm wf c m0 e.
+  { destruct c; simpl in e; inv e.
+    { exists Γ. exists [Γ]. exists Unit. exists U.
+      repeat split...
+      move=>k' Γ3 Γ' n mrg tyn//=.
+      have->//:=merge_pureR mrg (re_pure _). }
+    { have{ihm}[G1[G2[B0[t[mrg[tym0 ih]]]]]]:=ihm wf _ _ erefl.
+      exists G1. exists G2. exists B0. exists t.
+      repeat split... } }
+  move=>Γ m tym ihm wf c m0 e.
+  { destruct c; simpl in e; inv e.
+    { exists Γ. exists [Γ]. exists Unit. exists U.
+      repeat split...
+      move=>k' Γ3 Γ' n mrg tyn//=.
+      have->//:=merge_pureR mrg (re_pure _). }
+    { have{ihm}[G1[G2[B0[t[mrg[tym0 ih]]]]]]:=ihm wf _ _ erefl.
+      exists G1. exists G2. exists B0. exists t.
+      repeat split... } }
+  move=>Γ A B m s i sb tym ihm tyB _ wf c m0 e.
+  { have{ihm}[G1[G2[B0[t[mrg[tym0 ih]]]]]]:=ihm wf _ _ e.
+    exists G1. exists G2. exists B0. exists t.
+    repeat split...
+    move=>k' Γ3 Γ' n mrg' tyn.
+    have{}ih:=ih k' _ _ _ mrg' tyn.
+    have[_[e1 e2]]:=merge_re_re mrg.
+    have[_[e3 e4]]:=merge_re_re mrg'.
+    apply: clc_conv.
+    exact: sb.
+    exact: ih.
+    rewrite<-e4. rewrite e2... }
+Qed.
